Coq/src/SimRelCertStep.v
@@ -985,7 +985,7 @@ Section SimRelCertStepProps.
       { eapply basic_step_simrel_cont; eauto; apply SRCC. }
       { eapply simrel_cert_step_e2a; eauto. }
       { eapply Execution.step_preserves; eauto. apply SRCC. }
-      1-4 : admit.
+      1-5 : admit.
       (* jfe_ex_iss : dom_rel Sjfe ⊆₁ dom_rel (Sew ⨾ ⦗ X ∩₁ e2a ⋄₁ I ⦘) *)
       { arewrite (X ∩₁ e2a S' ⋄₁ I ≡₁ X ∩₁ e2a S ⋄₁ I ).
         { admit. }
